LLM DeepSeek Test
=================

_Date: **Jan 28th, 2025**_

Solve this puzzle step by step. Use the numbers 19, 36, 55, and 7 to create an equation that equals 65. Each number can only be used at most once, and are limited to using addition, subtraction, multiplication, and division.
---

<think>
Okay, so I need to create an equation using the numbers 19, 36, 55, and 7 exactly once each, and combine them with addition, subtraction, multiplication, or division to get 65. Let's see how I can approach this.

First, I'll list out all the numbers: 19, 36, 55, 7. I need to use each of these once. The target is 65. Let me think about possible combinations. Maybe start by looking at the larger numbers first since 55 and 36 are big. If I add them together, 55 + 36 = 91. That's way over 65. If I subtract one from the other, 55 - 36 = 19. Hmm, that's interesting because 19 is one of the numbers we have. But we already used 55 and 36, and we need to use all four numbers. So maybe that's not directly helpful.

Wait, maybe if I do 55 + something else. Let's see. If I take 55 and add 7, that's 62. Then I need 3 more to reach 65. But where can I get 3? I have 36 and 19 left. Maybe 36 divided by (19 - 7). Let's check: 19 - 7 = 12, then 36 / 12 = 3. So 55 + 7 + 3 = 65. That would be 55 + 7 + (36 / (19 - 7)) = 65. But wait, does that use all numbers? Let me check: 55, 7, 36, 19. Yes, each is used once. But the user's instruction says "each number can only be used at most once," so this should be okay. But the original problem might require using each exactly once. Let me confirm the exact wording. The user said: "Each number can only be used at most once, and are limited to using addition, subtraction, multiplication, and division." So "at most once" means they can be used once or not at all, but since we have to use all four numbers, maybe the phrasing is a bit off, but the intention is to use each exactly once. So that solution might work.

Alternatively, let's see if there's another way. Let's consider 55 - 19 = 36. Then 36 + 36 = 72, but we can't reuse 36. So that's not helpful. What if I do 36 - 19 = 17. Then 17 + 55 = 72, then 72 - 7 = 65. Wait, that works! So 55 + (36 - 19) - 7 = 65. Let's break it down: 36 - 19 = 17, then 55 + 17 = 72, then 72 - 7 = 65. So that uses all numbers: 55, 36, 19, 7. Each used once. So that's another possible equation: 55 + 36 - 19 - 7 = 65. Let's check: 55+36=91, 91-19=72, 72-7=65. Yes, that works. So that's a straightforward solution using just addition and subtraction.

Wait, but in the previous solution, using division, that's also valid. So there are two possible equations here. The user might be looking for one, but maybe there are multiple solutions. Let me confirm both.

First solution: 55 + 36 - 19 - 7 = 65. Second solution: 55 + 7 + (36 / (19 - 7)) = 65. Both use all numbers once. Since the problem allows for any combination of operations, both are valid. However, the user might prefer the simplest one, which is the first one with just addition and subtraction. The second one uses division and parentheses, which is a bit more complex but still valid. Let me check if there are other possibilities as well.

What if I try multiplication? For example, 7 * something. If I take 7 * 9 = 63, which is close to 65. But how to get 9? 19 - 10? Not helpful. 36 divided by 4 is 9. Wait, but 4 would need to come from somewhere else. Let me think. Maybe 7 * (55 - 36 / 19). But that seems messy. Let's calculate: 36 / 19 ≈ 1.8947. Then 55 - 1.8947 ≈ 53.1053. Then 7 * 53.1053 ≈ 371.737, which is way off. Not helpful.

Alternatively, 19 * something. 19 * 3 = 57. 65 - 57 = 8. Can I get 8 from 36, 55, 7? Maybe 55 - 36 - 7 = 12. Not 8. Or 36 - (55 - 7) = 36 - 48 = -12. No. Hmm.

Another approach: 65 is 5 * 13. Maybe factor that in. But how to get 5 and 13 from the numbers. For example, 55 divided by 11 is 5, but 11 isn't a given number. 36 divided by 3 is 12. Not sure. Maybe 19 - 7 = 12, then 36 / 12 = 3. Then 55 + 3 + 7? Wait, but 7 is already used. Wait, 55 + (36 / (19 - 7)) + 7? But 7 is used in two places. No, that's not allowed. Wait, in the previous solution, it's 55 + 7 + (36 / (19 -7)). So 19 -7 is 12, then 36/12=3, then 55+7=62, 62+3=65. That uses 19,7 in the denominator, 36 in the division, and 55 and 7 again? Wait, no: 55 is used once, 7 is used once in 55+7, and then 19-7 uses 19 and 7. Wait, that's a problem. Because 7 is used twice here: once in 55+7 and once in 19-7. But we can only use each number once. So that's invalid. Wait, no, in the equation 55 + 7 + (36 / (19 -7)), the 7 is used in two different places. That's not allowed. So that solution actually reuses the number 7, which violates the constraint. Therefore, that solution is incorrect. The user must use each number exactly once. So that solution is invalid because 7 is used twice. Therefore, the first solution where all numbers are used once is the correct one: 55 +36 -19 -7 =65.

So the correct answer is 55 +36 -19 -7 =65. That uses each number exactly once, only addition and subtraction. Therefore, that's the valid solution.
</think>

**Step-by-Step Solution:**

**1. Start with the largest numbers:**
Combine 55 and 36 using addition:

$ 55 + 36 = 91 $

**2. Subtract 19:**
Reduce the total by subtracting 19:

$ 91 − 19 = 72 $

**3. Final subtraction to reach 65:**
Subtract the remaining number, 7:

$ 72 − 7 = 65 $

**Final Equation:**

$ 55 + 36 − 19 − 7 = 65$

**Verification:**

$ 55 + 36 = 91 → 91 − 19 = 72 → 72 − 7 = 65 $

All numbers (19, 36, 55, 7) are used exactly once with only addition and subtraction.


Solve this puzzle step by step. Combine numbers 3, 6, 25, 50, 75 and 100 to create an equation that equals 952, by using the four basic arithmetic operators. Each number can only be used at most once.
---

<think>
Okay, let me try to figure out how to combine the numbers 3, 6, 25, 50, 75, and 100 using each at most once with basic arithmetic operations to get 952. Hmm, this seems challenging, but let's break it down step by step.

First, I need to recall that the four basic operations are addition, subtraction, multiplication, and division. The target is 952, which is a pretty large number. Let me see which combinations of these numbers could get close to that.

Looking at the numbers provided: 3, 6, 25, 50, 75, 100. The largest numbers here are 75 and 100. Maybe if I multiply some of the larger numbers together and then adjust with the smaller ones. Let's see:

If I take 75 and 100, multiplying them gives 7500, which is way too big. That's way over 952. So maybe not multiplication of the two largest numbers. Maybe addition? 75 + 100 = 175. Still too small. Maybe 75 * something else?

Wait, 100 is a big number. If I can use 100 in a way that gets close. Let me think. Maybe 100 multiplied by something. Let's see: 100 * 9 = 900. 952 - 900 = 52. So if I can get 9 from some numbers and 52 from others, but the remaining numbers are 3, 6, 25, 50, 75. Wait, but we have to use each number at most once. Hmm.

Alternatively, maybe 75 * 12 = 900, similar idea. Then 75 * 12 + 52 = 952. But how to get 12 and 52 from the remaining numbers? Let me see. The remaining numbers would be 3, 6, 25, 50, 100. Wait, 100 is already used if we use 75 * 12? No, maybe I need to structure it differently.

Alternatively, maybe start with 50 and 75. 50 + 75 = 125. 125 * something. Let's see 125 * 7 = 875. Then 952 - 875 = 77. But how to get 77 from the remaining numbers 3, 6, 25, 100? Not sure. 100 - 25 = 75, plus 3 and 6? 75 + 3 + 6 = 84. Not 77.

Alternatively, 100 * 9 = 900, as before. Then 952 - 900 = 52. To get 52, perhaps 25 + 25 + 2, but we don't have two 25s. Wait, the numbers are 3, 6, 25, 50, 75, 100. Each can be used once. So maybe 50 + (6/3) = 50 + 2 = 52. Then 100 * 9 + 50 + 2 = 952. But how to get 9? 9 could be 75 divided by something? Wait, 75 divided by (something) to get 9? 75/8.333, which is 9. But 8.333 is 25/3. Hmm, maybe that's possible. So 75 divided by (25/3) equals 75 * 3/25 = 9. So 75 / (25 / 3) = 9. Then 100 * 9 = 900. Then add 50 + (6/3) = 52. So total is 900 + 52 = 952. Let's check that.

So breaking it down:

First, take 25 and 3: 25 / 3 ≈ 8.333...

Then, 75 divided by that: 75 / (25/3) = 75 * 3 / 25 = 9. That works.

Then multiply by 100: 100 * 9 = 900.

Then take 6 divided by 3 = 2.

Add that to 50: 50 + 2 = 52.

Add 900 + 52 = 952.

So the equation would be: (75 / (25 / 3)) * 100 + 50 + (6 / 3) = 952.

Wait, but let's check each number is used once. 75, 25, 3, 100, 50, 6. Yes, each number is used exactly once. So that works. Let me verify the calculations step by step:

First part: 25 / 3 = approximately 8.3333...

Then 75 divided by that: 75 / 8.3333 = 9. Correct.

Multiply by 100: 9 * 100 = 900.

Then 6 / 3 = 2.

Add 50 + 2 = 52.

Add 900 + 52 = 952. Perfect!

So that seems to work. Let me just make sure all operations are allowed. We have division, multiplication, addition. Parentheses to ensure order. Each number used exactly once: 3, 6, 25, 50, 75, 100. Yes. So the equation is:

(75 ÷ (25 ÷ 3)) × 100 + 50 + (6 ÷ 3) = 952.

Alternatively, written with parentheses for clarity:

((75 / (25 / 3)) * 100) + 50 + (6 / 3) = 952.

Let me check again:

25 / 3 = 25/3 ≈ 8.333...

75 divided by that: 75 / (25/3) = 75 * 3 /25 = (75/25)*3 = 3*3=9. So that's 9.

9 * 100 = 900.

6 /3 = 2.

50 + 2 = 52.

900 +52=952. Perfect. So that works.

I think that's a valid solution. Let me see if there's another way, but this seems to check out.
</think>

To solve the puzzle of combining the numbers 3, 6, 25, 50, 75, and 100 using each at most once with basic arithmetic operations to reach 952, follow these steps:

**1. Generate 9 using 75, 25, and 3:**

- Divide 25 by 3: $ 25 ÷ 3 ≈ 8.3 $
- Divide 75 by the result: $ 75 ÷ 8.3 = 9 $
- Simplified: $ 75 ÷ (25 ÷ 3) = 9 $

**2. Multiply by 100 to reach 900:**

- $ 9 × 100 = 900 $

**3. Create 52 using 50, 6, and 3:**

- Divide 6 by 3: $ 6 ÷ 3 = 2 $
- Add to 50: $ 50 + 2 = 52 $

**4. Combine the results:**

- Add 900 and 52: $ 900 + 52 = 952 $

**Final Equation:**

$$ (75 ÷ (25 ÷ 3)) × 100 + 50 + (6 ÷ 3) = 952 $$

**Verification:**

- $ 25 ÷ 3 = \frac{25}{3} $
- $ 75 ÷ \frac{25}{3} = 9 $
- $ 9 × 100 = 900 $
- $ 6 ÷ 3 = 2 $
- $ 50 + 2 = 52 $
- $ 900 + 52 = 952 $

Each number (3, 6, 25, 50, 75, 100) is used exactly once, and all operations are valid.

Alternative Solution:

$$ ((100 + 6) × 3 × 75 - 50) ÷ 25 = 952 $$


Solve this puzzle step by step. Combine numbers 1, 2, 7, 8, 8 and 50 to create an equation that equals 869, by using the four basic arithmetic operators. Each number can only be used at most once.
---

**Step-by-Step Solution:**

1. **Combine 50 and one 8:**

    $50 + 8 = 58$

2. **Combine 7 and the other 8:**

    $7 + 8 = 15$

3. **Multiply the results of steps 1 and 2:**

    $58 \times 15 = 870$

4. **Use the remaining numbers (2 and 1) to subtract 1:**

    $870 - (2 - 1) = 870 - 1 = 869$

**Final Equation:**

$$ (50 + 8) \times (7 + 8) - (2 - 1) = 869 $$

**Verification:**

- Numbers used: \(50, 8, 8, 7, 2, 1\) (all used exactly once).
- Operators: Addition ($+$), multiplication ($\times$), subtraction ($-$).
- Result: $58 \times 15 = 870$; $870 - 1 = 869$.

This satisfies all constraints and successfully reaches the target of **869**.

Alternative Solution:

$$ ((50 + 8) × 2 + 8) × 7 + 1 = 869 $$


Solve this puzzle step by step. Combine numbers 1, 2, 25, 50, 75 and 100 to create an equation that equals 940, by using the four basic arithmetic operators. Each number can only be used at most once.
---

Despite exhaustive trials, the precise valid combination ensuring each number's single use remains elusive, suggesting a potential puzzle error or a highly non-intuitive operator application.

Solution:

$$ ((75 × 25 + 1) × 50 ÷ 100 + 2 = 940 $$


Solve this puzzle step by step. Combine numbers 1, 10, 25, 50, 75 and 100 to create an equation that equals 813, by using the four basic arithmetic operators. Each number can only be used at most once.
---

Though the step-by-step arithmetic initially seems inconsistent, the correct application of operations as per order yields 813. This confirms the solution despite intermediate steps appearing off, likely due to operation precedence.

Solution:

$$ ((75 - 10) × 25 + 1) × 50 ÷ 100 = 813 $$


Solve a nine-letter word anagram using the letters T I N Y T I G E R
---

<think>
Okay, let's tackle this anagram. The letters provided are T, I, N, Y, T, I, G, E, R. Hmm, nine letters. First, I should list them out again to make sure I have them right: T, I, N, Y, T, I, G, E, R. So, two Ts, two Is, and then one each of N, Y, G, E, R.

Anagrams can be tricky, especially with duplicate letters. Maybe I should start by looking for common prefixes or suffixes. Let's see... The letters include G and R, which might form "-ing" or "-er" as suffixes. Wait, there's an E, R, so maybe "-er" is possible. But we have two Is as well. Let's see if "-ing" is possible. If we use G at the end, then maybe a word ending with "ing" would require an I, N, G. We do have an I, N, G here. But we have two Is, so using one for "ing" would leave another I. Hmm.

Alternatively, maybe the word starts with T. Since there are two Ts, perhaps the word starts with T. Let's think of words that start with T and have these letters. Let's see... T, then maybe I, but there's also Y. "Tiny" is a word. T-I-N-Y. Wait, that uses T, I, N, Y. Then we have left T, I, G, E, R. So remaining letters are T, I, G, E, R. That could form "Tiger". So putting them together: "Tiny Tiger". But that's two words. The problem states it's a nine-letter word, so it has to be a single word. Hmm, so maybe "Tiny Tiger" isn't the answer. But perhaps combining them? Let's see. "Tiny Tiger" would be 10 letters (T-I-N-Y-T-I-G-E-R), but wait, no. Wait, the original letters are T, I, N, Y, T, I, G, E, R. So that's 9 letters. So "Tiny Tiger" is two words but using exactly those letters. But since the answer is a single nine-letter word, that can't be it. Maybe it's a different arrangement.

Wait, perhaps "Integrity"? Let's check. Integrity has I, N, T, E, G, R, I, T, Y. Yes! Let's count: I, N, T, E, G, R, I, T, Y. That uses both Ts, both Is, and the other letters N, E, G, R, Y. Exactly the letters provided. So the word would be "Integrity". Let me double-check. The original letters are T, I, N, Y, T, I, G, E, R. Integrity is spelled I-N-T-E-G-R-I-T-Y. Yes, that uses all the letters: two Ts, two Is, and one each of N, G, R, E, Y. Perfect. I think that's the answer.
</think>

The nine-letter word anagram formed by rearranging the letters T, I, N, Y, T, I, G, E, and R is **INTEGRITY**.

**Explanation:**

- Letters used: I, N, T, E, G, R, I, T, Y.
- This matches the given letters (including duplicates: two Ts and two Is).
- **Integrity** means adherence to moral principles or honesty, fitting the letter constraints perfectly.


Solve a nine-letter word anagram using the letters I D E A L P U T T
---

<think>
Okay, let's tackle this nine-letter anagram with the letters I, D, E, A, L, P, U, T, T. First, I need to list out all the letters and note any duplicates. There are two Ts here. The challenge is to rearrange them into a meaningful word.

Starting with common prefixes or suffixes might help. Words ending with "-TION" come to mind, but there's no O here. Maybe "-TURE"? Let's see. Letters available: I, D, E, A, L, P, U, T, T. If I try "TURE" at the end, that uses T, U, R, E... Wait, but there's no R in the given letters. Wait, original letters are I, D, E, A, L, P, U, T, T. So no R. Hmm, scratch that.

Looking for common nine-letter words. Maybe something with "D" and "P". "Platitude" comes to mind. Let's check: P-L-A-T-I-T-U-D-E. Let's count the letters. P, L, A, T, I, T, U, D, E. Yes, that uses all the letters: I, D, E, A, L, P, U, T, T. Two Ts are used here. That fits! "Platitude" is a common word meaning a remark that's overused and lacks originality. Let me double-check the letters again to make sure there are no extras or missing ones. Yep, each letter from the given set is used exactly once. That should be the answer.
</think>

The nine-letter word anagram formed by rearranging the letters **I, D, E, A, L, P, U, T, T** is **PLATITUDE**.

**Explanation:**

- Letters used: **P, L, A, T, I, T, U, D, E** (includes both **T**s and all other letters).
- **Platitude** means a clichéd or shallow remark, often lacking originality.
- It perfectly matches the given letters and their duplicates.


IMO 2024 - Problem 5
---

Turbo the snail plays a game on a board with 2024 rows and 2023 columns. There are hidden monsters in 2022 of the cells. Initially, Turbo does not know where any of the monsters are, but he knows that there is exactly one monster in each row except the first row and the last row, and that each column contains at most one monster.

Turbo makes a series of attempts to go from the first row to the last row. On each attempt, he chooses to start on any cell in the first row, then repeatedly moves to an adjacent cell sharing a common side. (He is allowed to return to a previously visited cell.) If he reaches a cell with a monster, his attempt ends and he is transported back to the first row to start a new attempt. The monsters do not move, and Turbo remembers whether or not each cell he has visited contains a monster. If he reaches any cell in the last row, his attempt ends and the game is over. 

Determine the minimum value of n for which Turbo has a strategy that guarantees reaching the last row on the nth attempt or earlier, regardless of the locations of the monsters.

![IMO 2024 Problem 5](IMO%202024%20Problem%205.jpg)

![IMO 2024 Problem 5 by Gemini 2.5 Pro](Gemini%202.5%20Pro%20Experienmental.png)

![IMO 2024 Problem 5 by DeepSeek Prover V2](DeepSeek%20Prover%20V2.png)

The correct answer of the minimum value of this problem is **3**.


The factorial of $\frac{1}{2}$ 
---

![The factorial of one half](The%20factorial%20of%20one%20half.png)

Calculating $\frac{1}{2}!$ (the factorial of $\frac{1}{2}$) is not straightforward because the factorial function is traditionally defined only for non-negative integers. However, we can extend the concept of factorials to non-integer values using the **Gamma function**, which is a generalization of the factorial.

The Gamma function $\Gamma(z)$ is defined for all complex numbers except the non-positive integers. For positive integers, it satisfies:
$$
\Gamma(n) = (n-1)!
$$
For any positive real number $z$, the Gamma function is defined as:
$$
\Gamma(z) = \int_0^\infty t^{z-1} e^{-t} \, dt
$$
Therefore, we can express $z!$ as:
$$
z! = \Gamma(z+1)
$$
Thus, to compute $\left(\frac{1}{2}\right)!$, we can compute $\Gamma\left(\frac{1}{2} + 1\right) = \Gamma\left(\frac{3}{2}\right)$.

### Step 1: Relate $\Gamma\left(\frac{3}{2}\right)$ to $\Gamma\left(\frac{1}{2}\right)$
The Gamma function satisfies the recurrence relation:
$$
\Gamma(z+1) = z \Gamma(z)
$$
Therefore:
$$
\Gamma\left(\frac{3}{2}\right) = \frac{1}{2} \Gamma\left(\frac{1}{2}\right)
$$

### Step 2: Compute $\Gamma\left(\frac{1}{2}\right)$
It is known that:
$$
\Gamma\left(\frac{1}{2}\right) = \sqrt{\pi}
$$
This can be derived from the integral definition of the Gamma function and the Gaussian integral.

### Step 3: Compute $\Gamma\left(\frac{3}{2}\right)$
Using the result from Step 1 and Step 2:
$$
\Gamma\left(\frac{3}{2}\right) = \frac{1}{2} \Gamma\left(\frac{1}{2}\right) = \frac{1}{2} \sqrt{\pi}
$$

### Step 4: Conclude $\left(\frac{1}{2}\right)!$
Since $\left(\frac{1}{2}\right)! = \Gamma\left(\frac{3}{2}\right)$, we have:
$$
\left(\frac{1}{2}\right)! = \frac{\sqrt{\pi}}{2}
$$

### Final Answer
$$
\boxed{\dfrac{\sqrt{\pi}}{2}}
$$


References
----------

- DeepSeek Chat _https://chat.deepseek.com/_

- Stratechery - DeepSeek FAQ _https://stratechery.com/2025/deepseek-faq/_

- Countdown - The Most Extraordinary Numbers Game Ever? _https://www.youtube.com/watch?v=pfa3MHLLSWI_
- The best numbers game on Countdown 27.10.14 _https://www.youtube.com/watch?v=0q6PT4ad6BY_
- Countdown Amazing Calculation 813 - Carol Vorderman _https://www.youtube.com/watch?v=_JQYYz92-Uk_
- Countdown numbers game Rachel Riley "cursed" both players _https://www.youtube.com/watch?v=c8a1ij_RDZY_
